

MATH 440 Homework 6

Chris Camano: ccamano@sfsu.edu

3/10/2022

3.4.6

Let n be positive integer, show that $f(y) = (n+2)(n+1)y^n(1-y), 0 \leq y \leq 1$ is a pdf

$$\begin{aligned}\int_0^1 (n+2)(n+1)y^n(1-y)dy &= 1 \\(n+2)(n+1) \int_0^1 y^n(1-y)dy &= 1 \\(n+2)(n+1) \int_0^1 y^n - y^{n+1}dy &= 1 \\(n+2)(n+1) \left[\int_0^1 y^n dy - \int_0^1 y^{n+1} dy \right] &= 1 \\(n+2)(n+1) \left[\frac{y^{n+1}}{n+1} \Big|_0^1 - \frac{y^{n+2}}{n+2} \Big|_0^1 \right] &= 1 \\(n+2)(n+1) \left[\frac{1}{n+1} - \frac{1}{n+2} \right] &= 1 \\(n+2)(n+1) \left[\frac{n+2-n+1}{(n+1)(n+2)} \right] &= 1 \\n+2-n+1 &= 1 \\1 &= 1\end{aligned}$$

3.4.9

$$F_Y(y) = \int_{-\infty}^y f_Y(t) dy$$

$$\forall y > 0$$

$$F_Y(y) = \int_{-1}^y 1 - |t| dt$$

$$\int_{-1}^0 1 + t dt + \int_0^y 1 - t dt$$

$$F_Y(y) = (t + \frac{t^2}{2} \Big|_{-1}^0) + (t - \frac{t^2}{2} \Big|_0^y)$$

$$F_Y(y) = 1 - \frac{1}{2} + y - \frac{y^2}{2}$$

$$\forall y \leq 0$$

$$F_Y(y) = \int_{-1}^y 1 - |t| dt$$

$$\int_{-1}^y 1 + t dt$$

$$F_Y(y) = t + \frac{t^2}{2} \Big|_{-1}^y$$

$$F_Y(y) = \frac{1}{2} + y + \frac{y^2}{2}$$

Thus, $F_Y(y)=0 \quad \forall y < -1$

$$F_Y(y) = \frac{1}{2} + y + \frac{y^2}{2} \quad \forall y, -1 \leq y \leq 0$$

$$F_Y(y) = 1 - \frac{1}{2} + y - \frac{y^2}{2} \quad \forall y, 0 < y \leq 1$$

and 1 for all y greater than one

3.4.14

$$F_Y(y) = \int_0^y te^{-t} dt$$

$$\text{let } u = t, du = 1, dv = e^{-t}, v = -e^{-t}$$

$$F_Y(y) = \int_0^y te^{-t} dt = -te^{-t} + \int e^{-t} dt$$

$$F_Y(y) = \int_0^y te^{-t} dt = -te^{-t} - e^{-t}$$

$$F_Y(y) = -te^{-t} - e^{-t} \Big|_0^y$$

$$F_Y(y) = -ye^{-y} - e^{-y} + 1)$$